TreeSem.thy
@@ -1,0 +1,240 @@
+theory TreeSem
+  imports Soundness "HOL-Cardinals.Bounded_Set"
+begin
+
+section \<open> Bounded Set Utils \<close>
+
+lemma bmember_bmap_iff:
+  \<open>bmember y (map_bset f B) \<longleftrightarrow> (\<exists>x. bmember x B \<and> y = f x)\<close>
+  by transfer (force simp add: image_def)
+
+lemma bCollect_eq_bempty_iff:
+  \<open>bCollect p = bempty \<longleftrightarrow> (\<nexists>x. p x)\<close>
+  by (metis Collect_empty_eq bCollect.rep_eq bempty.rep_eq set_bset_inject)
+
+lemma pred_bset_bempty[simp]:
+  \<open>pred_bset p bempty\<close>
+  by (simp add: bset.pred_rel)
+
+lemma pred_bCollect_eq[simp]:
+  \<open>pred_bset p (bCollect q) = (q \<le> p)\<close>
+  by (simp add: bCollect.rep_eq bset.pred_set le_fun_def)
+
+section \<open> Semantic Trees \<close>
+
+datatype 'a label = Env | Local \<open>'a act\<close>
+
+datatype ('c, 's, 'l) sem_tree =
+  Branch
+    (config_sem_tree: \<open>'s \<times> 'c\<close>)
+    (branches_sem_tree:
+      \<open>('l \<times> (('c, 's, 'l) sem_tree + unit)) set[('l \<times> (('s + unit) \<times> 'c)) set]\<close>)
+
+lemma sem_tree_induct:
+  \<open>(\<And>ty.
+      (\<And>l tx.
+        (l, Inl tx) \<in> set_bset (branches_sem_tree ty) \<Longrightarrow>
+        P tx) \<Longrightarrow>
+      P ty) \<Longrightarrow>
+    P t\<close>
+  apply (rule sem_tree.induct)
+  apply (clarsimp simp add: image_def Bex_def)
+  apply (metis sem_tree.sel(2) setl.intros)
+  done
+
+function pred_sem_tree
+  :: \<open>('s \<times> 'c \<Rightarrow> bool) \<Rightarrow> ('c, 's, 'l) sem_tree \<Rightarrow> bool\<close>
+  where
+  \<open>pred_sem_tree p (Branch sc S) =
+    (p sc \<and> pred_bset (\<lambda>v. case v of (l,mt') \<Rightarrow> case_sum (pred_sem_tree p) (\<lambda>_. False) mt') S)\<close>
+  by pat_completeness auto
+termination
+  apply (relation
+      \<open>{((xa,ta),(xb,tb)). xa = xb \<and> (\<exists>l. (l, Inl ta) \<in> set_bset (branches_sem_tree tb))}\<close>)
+   apply (clarsimp simp add: wf_def, rule sem_tree_induct, blast)
+  apply force
+  done
+
+function step_rel_sem_tree
+  :: \<open>('l \<Rightarrow> 's \<Rightarrow> 's + unit \<Rightarrow> bool) \<Rightarrow> ('c, 's, 'l) sem_tree \<Rightarrow> bool\<close>
+  where
+  \<open>step_rel_sem_tree r (Branch (s, c) S) =
+      pred_bset
+        (\<lambda>(l,mt'). r l s (map_sum (fst \<circ> config_sem_tree) id mt') \<and>
+                   (\<forall>t'. mt' = Inl t' \<longrightarrow> step_rel_sem_tree r t'))
+        S\<close>
+  by pat_completeness auto
+termination
+  apply (relation
+      \<open>{((xa,ta),(xb,tb)). xa = xb \<and> (\<exists>l. (l, Inl ta) \<in> set_bset (branches_sem_tree tb))}\<close>)
+   apply (clarsimp simp add: wf_def, rule sem_tree_induct, blast)
+  apply force
+  done
+
+
+function steps_pred_sem_tree
+  :: \<open>(('s \<times> 'l \<times> ('s + unit)) set \<Rightarrow> bool) \<Rightarrow> ('c, 's, 'l) sem_tree \<Rightarrow> bool\<close>
+  where
+  \<open>steps_pred_sem_tree p (Branch (s,c) S) =
+    (p (set_bset (map_bset (\<lambda>(l, mt'). (s, l, map_sum (fst \<circ> config_sem_tree) id mt')) S)) \<and>
+      pred_bset (\<lambda>v. \<forall>l t'. v = (l, Inl t') \<longrightarrow> steps_pred_sem_tree p t') S)\<close>
+  by pat_completeness auto
+termination
+  apply (relation
+      \<open>{((xa,ta),(xb,tb)). xa = xb \<and> (\<exists>l. (l, Inl ta) \<in> set_bset (branches_sem_tree tb))}\<close>)
+   apply (clarsimp simp add: wf_def, rule sem_tree_induct, blast)
+  apply force
+  done
+
+(*
+definition
+  \<open>sem_tree_contains t1 t2 \<equiv>
+    (t1, t2) \<in> {(t1,t2). t1 \<in> snd ` set_bset (branches_sem_tree t2)}\<^sup>+\<close>
+
+lemmas sem_tree_contains_baseI =
+  r_into_trancl[
+    of _ _ \<open>{(t1,t2). t1 \<in> snd ` set_bset (branches_sem_tree t2)}\<close>,
+    simplified,
+    simplified sem_tree_contains_def[symmetric]]
+
+lemmas sem_tree_contains_stepI =
+  trancl_into_trancl[
+    of _ _ \<open>{(t1,t2). t1 \<in> snd ` set_bset (branches_sem_tree t2)}\<close>,
+    simplified,
+    simplified sem_tree_contains_def[symmetric]]
+
+lemmas sem_tree_contains_induct =
+  trancl.induct[
+    of _ _ \<open>{(t1,t2). t1 \<in> snd ` set_bset (branches_sem_tree t2)}\<close>,
+    simplified,
+    simplified sem_tree_contains_def[symmetric]]
+
+lemmas sem_tree_containsE[elim] =
+  trancl.cases[
+    of _ _ \<open>{(t1,t2). t1 \<in> snd ` set_bset (branches_sem_tree t2)}\<close>,
+    simplified,
+    simplified sem_tree_contains_def[symmetric]]
+
+lemma sem_tree_contains_branches_no_loop:
+  \<open>sem_tree_contains a b \<Longrightarrow>
+    b \<notin> snd ` set_bset (branches_sem_tree a)\<close>
+  by (induct b arbitrary: a rule: sem_tree_induct)
+    (meson sem_tree_containsE sem_tree_contains_baseI trancl_trans
+      sem_tree_contains_def)
+
+lemma sem_tree_contains_no_loop:
+  \<open>sem_tree_contains a b \<Longrightarrow> \<not> sem_tree_contains b a\<close>
+  by (erule sem_tree_contains_induct)
+    (meson sem_tree_contains_branches_no_loop sem_tree_contains_def trancl_trans)+
+*)
+
+
+
+fun bounded_treesem
+  :: \<open>('s \<Rightarrow> 's \<Rightarrow> bool) \<Rightarrow>
+      ('l \<times> 's \<Rightarrow> bool) \<Rightarrow>
+      ('l::pre_perm_alg \<times> 's) \<times> ('l \<times> 's, unit) comm \<Rightarrow>
+      nat \<Rightarrow>
+      (('l \<times> 's, unit) comm, 'l \<times> 's, unit label) sem_tree\<close>
+  where
+  \<open>bounded_treesem r F sc 0 = Branch sc bempty\<close>
+| \<open>bounded_treesem r F (s, c) (Suc n) =
+    Branch (s, c)
+      (map_bset (apsnd
+        (\<lambda>(z', c').
+          case z' of
+            Inl s' \<Rightarrow> Inl (bounded_treesem r F (s', c') n)
+          | Inr () \<Rightarrow> Inr ()))
+        (bCollect
+          (\<lambda>(l, (z', c')).
+              (\<exists>\<alpha>. l = Local \<alpha> \<and> (s, c) \<midarrow>\<alpha>\<rightarrow> (z', c')) \<or>
+              (\<exists>hs'. l = Env \<and> r (snd s) hs' \<and> z' = Inl (fst s, hs') \<and> c' = c))))\<close>
+
+(* TODO: precondition limitations *)
+
+(*
+definition treesem
+  :: \<open>('s \<Rightarrow> 's \<Rightarrow> bool) \<Rightarrow>
+      ('l \<times> 's, unit) comm \<Rightarrow>
+      (('l \<times> 's, unit) comm, 'l \<times> 's, unit label) sem_tree set\<close> where
+  \<open>treesem r c \<equiv> range (bounded_treesem r c)\<close>
+*)
+
+
+definition sem_tree_nocrash
+  :: \<open>(('l \<times> 's, unit) comm, 'l \<times> 's, unit label) sem_tree \<Rightarrow> bool\<close>
+  where
+  \<open>sem_tree_nocrash \<equiv> step_rel_sem_tree (\<lambda>_ _ z'. z' \<noteq> Inr ())\<close>
+
+definition sem_tree_post
+  :: \<open>('s \<Rightarrow> bool) \<Rightarrow>
+      (('s, unit) comm, 's, unit label) sem_tree \<Rightarrow>
+      bool\<close>
+  where
+  \<open>sem_tree_post q \<equiv> pred_sem_tree (\<lambda>(s,c). c = Skip \<longrightarrow> q s)\<close>
+
+definition sem_tree_guar
+  :: \<open>('s \<Rightarrow> 's \<Rightarrow> bool) \<Rightarrow>
+      (('l \<times> 's, unit) comm, 'l \<times> 's, unit label) sem_tree \<Rightarrow>
+      bool\<close>
+  where
+  \<open>sem_tree_guar g \<equiv>
+    step_rel_sem_tree (\<lambda>l s z'. \<forall>\<alpha> s'. l = Local \<alpha> \<longrightarrow> z' = Inl s' \<longrightarrow> g (snd s) (snd s'))\<close>
+
+definition sem_tree_states
+  :: \<open>('l \<times> 's \<Rightarrow> bool) \<Rightarrow>
+      (('l \<times> 's, unit) comm, 'l \<times> 's, unit label) sem_tree \<Rightarrow>
+      bool\<close>
+  where
+  \<open>sem_tree_states S \<equiv> pred_sem_tree (S \<circ> fst)\<close>
+
+definition sem_tree_frame_cond
+  :: \<open>('l::pre_perm_alg \<times> 's \<Rightarrow> bool) \<Rightarrow>
+      (('l \<times> 's, unit) comm, 'l \<times> 's, unit label) sem_tree \<Rightarrow>
+      bool\<close>
+  where
+  \<open>sem_tree_frame_cond F \<equiv>
+    steps_pred_sem_tree (\<lambda>S.
+      \<forall>\<alpha> hl hs hl' hs'.
+        ((hl, hs), Local \<alpha>, (Inl (hl', hs'))) \<in> S \<longrightarrow>
+        (\<forall>hlf hlhlf'.
+          F (hlf, hs) \<longrightarrow>
+          hl ## hlf \<longrightarrow>
+          ((hl + hlf, hs), Local \<alpha>, (Inl (hlhlf', hs'))) \<in> S \<longrightarrow>
+          (\<exists>hl'. hl' ## hlf \<and> hlhlf' = hl' + hlf)))\<close>
+
+
+definition sem_tree_safe
+  :: \<open>('l::pre_perm_alg \<times> 's \<Rightarrow> bool) \<Rightarrow>
+      ('s \<Rightarrow> 's \<Rightarrow> bool) \<Rightarrow>
+      ('l \<times> 's \<Rightarrow> bool) \<Rightarrow>
+      (('l \<times> 's, unit) comm, 'l \<times> 's, unit label) sem_tree \<Rightarrow>
+      bool\<close>
+  where
+  \<open>sem_tree_safe q g S \<equiv>
+    sem_tree_nocrash \<sqinter>
+    sem_tree_post q \<sqinter>
+    sem_tree_guar g \<sqinter>
+    sem_tree_states S\<close>
+
+
+lemma safe_then_sem_tree_safe:
+  \<open>safe n c z r g q S F \<Longrightarrow>
+    z = Inl s \<Longrightarrow>
+    sem_tree_safe q g S (bounded_treesem r F (s, c) n)\<close>
+  apply (induct arbitrary: s rule: safe.inducts)
+  sorry
+
+lemma sem_tree_safe_then_safe:
+  \<open>sem_tree_safe q g S (bounded_treesem r F (s, c) n) \<Longrightarrow>
+    safe n c (Inl s) r g q S F\<close>
+  apply (induct n arbitrary: s c)
+  sorry
+
+theorem safe_iff_sem_tree_safe:
+  \<open>safe n c (Inl s) r g q S F \<longleftrightarrow> sem_tree_safe q g S (bounded_treesem r F (s, c) n)\<close>
+  using safe_then_sem_tree_safe sem_tree_safe_then_safe
+  by fast
+
+
+end
